WIP locals

ch2o_compcertc_lp64.v
@@ -12,36 +12,54 @@ Local Open Scope string_scope.
 
 Context (Γ: types.env K) (δ: funenv K) (p: Csyntax.program).
 
-Inductive expr_equiv: expressions.expr K → Csyntax.expr → Prop :=
+Notation tint := (Tint I32 Signed noattr).
+
+Inductive type_ := Int | Loc.
+
+Inductive expr_equiv(ê: list AST.ident): expressions.expr K → Csyntax.expr → type_ → Prop :=
 | expr_equiv_val_int z:
   int_typed z (sintT: int_type K) → (* TODO: Require the CH2O program to be well-typed instead? *)
-  expr_equiv (EVal ∅ (inr (intV{sintT} z))) (Eval (Vint (Int.repr z)) (Tint I32 Signed noattr))
+  expr_equiv ê (# intV{sintT} z) (Eval (Vint (Int.repr z)) tint) Int
 | expr_equiv_div e1 ė1 e2 ė2:
-  expr_equiv e1 ė1 →
-  expr_equiv e2 ė2 →
-  expr_equiv (e1 / e2) (Ebinop Odiv ė1 ė2 (Tint I32 Signed noattr))
+  expr_equiv ê e1 ė1 Int →
+  expr_equiv ê e2 ė2 Int →
+  expr_equiv ê (e1 / e2) (Ebinop Odiv ė1 ė2 tint) Int
+| expr_equiv_var i x:
+  ê !! i = Some x →
+  expr_equiv ê (var i) (Evar x tint) Loc
+| expr_equiv_loc b:
+  expr_equiv ê (%(Ptr (addr_top (Npos b) sintT))) (Eloc b Ptrofs.zero tint) Loc
+| expr_equiv_load e ė:
+  expr_equiv ê e ė Loc →
+  expr_equiv ê (load e)%E (Evalof ė tint) Int
+| expr_equiv_val_indet:
+  expr_equiv ê (# indetV sintT) (Eval Vundef tint) Int
 .
 
-Inductive stmt_equiv: stmt K → statement → Prop :=
+Inductive stmt_equiv(ê: list AST.ident): stmt K → statement → Prop :=
 | stmt_equiv_return e ė:
-  expr_equiv e ė →
-  stmt_equiv (ret (cast{sintT%T} e)) (Sreturn (Some ė))
+  expr_equiv ê e ė Int →
+  stmt_equiv ê (ret (cast{sintT%T} e)) (Sreturn (Some ė))
 | stmt_equiv_skip:
-  stmt_equiv SSkip Sskip
+  stmt_equiv ê skip Sskip
 | stmt_equiv_sequence s1 ṡ1 s2 ṡ2:
-  stmt_equiv s1 ṡ1 →
-  stmt_equiv s2 ṡ2 →
-  stmt_equiv (SComp s1 s2) (Ssequence ṡ1 ṡ2)
+  stmt_equiv ê s1 ṡ1 →
+  stmt_equiv ê s2 ṡ2 →
+  stmt_equiv ê (s1 ;; s2) (Ssequence ṡ1 ṡ2)
 | stmt_equiv_if e ė s1 ṡ1 s2 ṡ2:
-  expr_equiv e ė →
-  stmt_equiv s1 ṡ1 →
-  stmt_equiv s2 ṡ2 →
-  stmt_equiv (SIf e s1 s2) (Sifthenelse ė ṡ1 ṡ2)
+  expr_equiv ê e ė Int →
+  stmt_equiv ê s1 ṡ1 →
+  stmt_equiv ê s2 ṡ2 →
+  stmt_equiv ê (if{e} s1 else s2) (Sifthenelse ė ṡ1 ṡ2)
+| stmt_equiv_assign i x e ė:
+  ê !! i = Some x →
+  expr_equiv ê e ė Int →
+  stmt_equiv ê (! (cast{voidT%T} (var i) ::= e)) (Sdo (Eassign (Evar x tint) ė tint))
 .
 
 Inductive program_equiv: Prop :=
-| program_equiv_intro s ṡ b:
-  stringmap_lookup "main" δ = Some s →
+| program_equiv_intro ê s ṡ b:
+  stringmap_lookup "main" δ = Some (Nat.iter (length ê) (λ s, local{sintT} s) s) →
   Genv.init_mem p <> None →
   let ge := globalenv p in
   Genv.find_symbol ge p.(prog_main) = Some b →
@@ -49,14 +67,14 @@ Inductive program_equiv: Prop :=
     fn_return:=type_int32s;
     fn_callconv:=AST.cc_default;
     fn_params:=nil;
-    fn_vars:=nil;
+    fn_vars:=foldr (λ (x: AST.ident) xs, ((x, tint)::xs)) [] ê;
     fn_body:=
       Ssequence
-        ṡ
+        ṡ 
         (Sreturn (Some (Eval (Vint (Int.repr 0)) (Tint I32 Signed noattr))))
   |} in
   Genv.find_funct_ptr ge b = Some (Internal f) →
-  stmt_equiv s ṡ →
+  stmt_equiv ê s ṡ →
   program_equiv.
 
 Fixpoint globdef_is_fun{F V}(g: AST.globdef F V): bool :=
@@ -162,6 +180,7 @@ destruct (classic (imm_safe (globalenv p) e RV a m)).
   + eassumption.
 Qed.
 
+(*
 Lemma expr_equiv_no_LV_context e ė:
   expr_equiv e ė →
   ∀ C a,
@@ -177,8 +196,7 @@ induction 1; intros.
   + injection H2; clear H2; intros; subst.
     eelim IHexpr_equiv2 with (1:=H3); reflexivity.
 Qed.
-
-Notation tint := (Tint I32 Signed noattr).
+*)
 
 Lemma sem_cast_int z m:
   sem_cast (Vint (Int.repr z)) tint tint m = Some (Vint (Int.repr z)).
@@ -210,27 +228,84 @@ simpl.
 reflexivity.
 Qed.
 
-Lemma rred_safe e ė:
-  expr_equiv e ė →
-  ∀ C a ẽ ṁ t a' ṁ' ρ m,
-  context RV RV C →
+Fixpoint ch2o_val_of(oz: option Z): val K :=
+  match oz with
+    None => indetV sintT
+  | Some z => intV{sintT} z
+  end.
+
+Fixpoint compcert_val_of(oz: option Z): Values.val :=
+  match oz with
+    None => Vundef
+  | Some z => Vint (Int.repr z)
+  end.
+
+Inductive block_equiv(m: memory_map.mem K)(ṁ: Memory.Mem.mem)(b: Values.block): Prop :=
+| block_equiv_not_alloced:
+  Memory.Mem.loadv AST.Mint32 ṁ (Vptr b Ptrofs.zero) = None →
+  (∀ v, Memory.Mem.storev AST.Mint32 ṁ (Vptr b Ptrofs.zero) v = None) →
+  Memory.Mem.free ṁ b 0%Z 4%Z = None →
+  m !!{Γ} addr_top (Npos b) sintT = None →
+  ~ mem_writable Γ (addr_top (Npos b) sintT) m →
+  block_equiv m ṁ b
+| block_equiv_alloced oz:
+  Memory.Mem.loadv AST.Mint32 ṁ (Vptr b Ptrofs.zero) = Some (compcert_val_of oz) →
+  (∀ z', Memory.Mem.storev AST.Mint32 ṁ (Vptr b Ptrofs.zero) (Vint (Int.repr z')) ≠ None) →
+  Memory.Mem.free ṁ b 0%Z 4%Z ≠ None →
+  m !!{Γ} addr_top (Npos b) sintT = Some (ch2o_val_of oz) →
+  mem_writable Γ (addr_top (Npos b) sintT) m →
+  match oz with None => True | Some z => int_typed z (sintT: int_type K) end →
+  block_equiv m ṁ b
+.
+
+Record mem_equiv(m: memory_map.mem K)(ṁ: Memory.Mem.mem) := {
+  blocks_equiv: ∀ b, block_equiv m ṁ b;
+  domains_equiv: ∀ b, (ṁ.(Memory.Mem.nextblock) ≤ b)%positive → (Npos b : index) ∉ dom indexset m
+}.
+
+Inductive env_equiv(ẽ: Csem.env): list AST.ident → list (index * types.type K) → Prop :=
+| env_equiv_nil:
+  env_equiv ẽ [] []
+| env_equiv_cons x ê b ρ:
+  Maps.PTree.get x ẽ = Some (b, tint) →
+  env_equiv ẽ ê ρ →
+  env_equiv ẽ (x::ê) ((Npos b, sintT%T)::ρ)
+.
+
+Inductive lrred: Csem.env → kind → expr → Memory.mem → Events.trace → expr → Memory.mem → Prop :=
+| lrred_lred ẽ a ṁ a' ṁ':
+  lred (globalenv p) ẽ a ṁ a' ṁ' →
+  lrred ẽ LV a ṁ Events.E0 a' ṁ'
+| lrred_rred ẽ a ṁ t a' ṁ':
+  rred (globalenv p) a ṁ t a' ṁ' →
+  lrred ẽ RV a ṁ t a' ṁ'
+.
+
+Lemma lrred_safe ê e ė θ:
+  expr_equiv ê e ė θ →
+  ∀ C K_ K_' a ẽ ṁ t a' ṁ' ρ m,
+  context K_ K_' C →
   ė = C a →
-  rred ẽ a ṁ t a' ṁ' →
+  lrred ẽ K_ a ṁ t a' ṁ' →
+  mem_equiv m ṁ →
+  env_equiv ẽ ê ρ →
   ∃ (E: ectx K) e1 e2,
   e = subst E e1 ∧
   Γ \ ρ ⊢ₕ e1, m ⇒ e2, m ∧
-  expr_equiv (subst E e2) (C a') ∧
+  expr_equiv ê (subst E e2) (C a') θ ∧
   ṁ' = ṁ.
 Proof.
 induction 1; intros.
 - inversion H0; clear H0; subst; try discriminate.
   subst.
-  inversion H2.
-- inversion H1; clear H1; subst; try discriminate.
+  inversion H2; clear H2; subst; inversion H0.
+- rename H4 into Hmem_equiv.
+  rename H5 into Menv_equiv.
+  inversion H1; clear H1; subst; try discriminate.
   + subst.
-    inversion H3; clear H3; subst.
-    inversion H; clear H; subst.
-    inversion H0; clear H0; subst.
+    inversion H3; clear H3; subst; inversion H1; clear H1; subst.
+    inversion H; clear H; subst;
+    inversion H0; clear H0; subst; try discriminate.
     simpl in H10.
     unfold sem_div in H10.
     unfold sem_binarith in H10.
@@ -423,7 +498,7 @@ induction 1; intros.
     }
     reflexivity.
   + injection H2; clear H2; intros; subst.
-    destruct (IHexpr_equiv1 C0 a ẽ ṁ t a' ṁ' ρ m H4) as [E [e5 [e6 [? [? ?]]]]]; try trivial.
+    destruct (IHexpr_equiv1 C0 K_ RV a ẽ ṁ t a' ṁ' ρ m H4) as [E [e5 [e6 [? [? ?]]]]]; try trivial.
     exists (E ++ [CBinOpL (ArithOp DivOp) e2])%E; eexists; eexists.
     rewrite subst_snoc.
     rewrite subst_snoc.
@@ -434,7 +509,7 @@ induction 1; intros.
     split. { constructor; tauto. }
     destruct H5; congruence.
   + injection H2; clear H2; intros; subst.
-    destruct (IHexpr_equiv2 C0 a ẽ ṁ t a' ṁ' ρ m H4) as [E [e5 [e6 [? [? [? Hṁ']]]]]]; try trivial.
+    destruct (IHexpr_equiv2 C0 K_ RV a ẽ ṁ t a' ṁ' ρ m H4) as [E [e5 [e6 [? [? [? Hṁ']]]]]]; try trivial.
     exists (E ++ [CBinOpR (ArithOp DivOp) e1])%E; eexists; eexists.
     rewrite subst_snoc.
     rewrite subst_snoc.
@@ -444,6 +519,94 @@ induction 1; intros.
     split. { apply H2. }
     split. { constructor; assumption. }
     assumption.
+- inversion H0; clear H0; subst; try discriminate.
+  subst.
+  inversion H2; clear H2; subst; inversion H0; clear H0; subst. 2:{
+    apply False_ind.
+    revert H4 i H.
+    induction 1; intros.
+    - discriminate.
+    - destruct i.
+      + simpl in H0.
+        injection H0; clear H0; intros; subst.
+        congruence.
+      + simpl in H0.
+        eapply IHenv_equiv; eassumption.
+  }
+  exists [].
+  exists (var i)%E.
+  exists (%(Ptr (addr_top (Npos b) sintT)))%E.
+  split. { reflexivity. }
+  split. {
+    constructor.
+    revert H4 i H.
+    induction 1; intros.
+    - discriminate.
+    - destruct i.
+      + simpl in H0.
+        injection H0; clear H0; intros; subst.
+        assert (b0 = b). congruence.
+        subst.
+        reflexivity.
+      + simpl in *.
+        apply IHenv_equiv; assumption.
+  }
+  split. {
+    constructor.
+  }
+  reflexivity.
+- inversion H; clear H; subst; try discriminate.
+  subst.
+  inversion H1; clear H1; subst; inversion H; clear H; subst.
+- inversion H0; clear H0; subst; try discriminate.
+  + subst.
+    inversion H2; clear H2; subst; inversion H0; clear H0; subst.
+    inversion H; clear H; subst.
+    inversion H9; clear H9; subst; try discriminate.
+    simpl in H.
+    injection H; clear H; intros; subst.
+    pose proof (blocks_equiv _ _ H3 b).
+    inversion H; clear H; subst; try congruence.
+    assert (v = compcert_val_of oz). congruence. subst.
+    exists []; eexists; eexists.
+    split. { reflexivity. }
+    split. {
+      assert (m = mem_force Γ (addr_top (N.pos b) sintT) m). {
+        unfold mem_force.
+        simpl.
+        unfold cmap_alter_ref.
+        destruct m.
+        simpl.
+        rewrite alter_id.
+        - reflexivity.
+        - intros.
+          unfold cmap_elem_map.
+          destruct x; reflexivity.
+      }
+      rewrite H at 2.
+      constructor.
+      eassumption.
+    }
+    split. {
+      destruct oz; constructor.
+      assumption.
+    }
+    reflexivity.
+  + injection H1; clear H1; intros; subst.
+    destruct (IHexpr_equiv _ _ _ _ _ _ _ _ _ _ _ H5 eq_refl H2 H3 H4) as [E [e1 [e2 [? [? [? ?]]]]]].
+    subst.
+    exists (E ++ [CLoad]); eexists; eexists.
+    rewrite ! subst_snoc.
+    split. { reflexivity. }
+    split. { eassumption. }
+    split. {
+      simpl.
+      constructor; assumption.
+    }
+    reflexivity.
+- inversion H; clear H; subst; try discriminate.
+  subst.
+  inversion H1; clear H1; subst; inversion H; clear H; subst.
 Qed.
 
 Lemma expr_equiv_no_call e ė:
